src/impl/TLS13.Impl.Server.Driver.Handshake.fsti
@@ -260,6 +260,48 @@ fn select_default_server_parameters_from_payload_once
               st1
               (Ghost.reveal 'payload_bytes))
 
+fn derive_shared_secret_from_payload_once
+  (d:DS.server_driver)
+  (payload:array U8.t)
+  (payload_len:SZ.t)
+  requires DS.server_driver_connected
+                d
+                'st0
+                'certificate_chain
+                'credential_identity
+                'received
+                'sent **
+           pts_to payload 'payload_bytes **
+           pure (B.length 'payload_bytes == SZ.v payload_len /\
+                   SZ.v payload_len == 32 /\
+                   ST.server_local_event_input_ready
+                     'st0
+                     ST.LocalDeriveSharedSecret
+                     (Ghost.reveal 'payload_bytes))
+  returns resp:ST.server_response
+  ensures exists* st1 sent'.
+          DS.server_driver_connected
+              d
+              st1
+              'certificate_chain
+              'credential_identity
+              'received
+              sent' **
+          pts_to payload 'payload_bytes **
+          pure (DL.server_driver_local_write_correct
+              'st0
+              st1
+              resp
+              ST.LocalDeriveSharedSecret
+              (Ghost.reveal 'payload_bytes)
+              (Ghost.reveal 'sent)
+              sent' /\
+           server_driver_derive_shared_secret_success_correct
+              'st0
+              st1
+              resp
+              (Ghost.reveal 'payload_bytes))
+
 fn accept_transport_and_start_once
   (d:DS.server_driver)
   (bind_host:array U8.t)
